AGM done

Algebraic_Group_Model.thy
@@ -1,9 +1,83 @@
 theory Algebraic_Group_Model 
-  imports Polynomial_Commitment_Schemes
+  imports CryptHOL.CryptHOL
   keywords
-  "lift_to_algebraic" :: thy_decl
-and  "local_test" :: thy_decl
+  "lift_to_agm" :: thy_decl
+and  "AGMtransform" :: thy_decl
 begin
+
+context cyclic_group
+begin 
+
+text \<open>check the rules of an algebraic algorithm i.e. given the elements g, agroup element, 
+and the vector vec_c=[c_0,...c_n] from the algorithm ensure that g=s_0 [^] c_0 \<otimes> ... \<otimes>
+s_0 [^] c_0, where [s_0,...,s_n]=seen are the group values the algorithm was supplied with.
+\<close>
+fun constrain :: "'a list \<Rightarrow> 'a \<Rightarrow> (int list) \<Rightarrow> bool"
+  where "constrain seen_vec g c_vec = (length seen_vec = length c_vec 
+    \<and> g = fold (\<lambda> i acc. acc \<otimes> seen_vec!i [^] (c_vec!i)) [0..<length seen_vec] \<one>)"
+
+text \<open>Given a list of group elements and vectors from an algebraic algorithm, 
+constrain all of them to the rules of algebraic algorithms\<close>
+fun constrain_list :: "'a list \<Rightarrow> ('a \<times> int list) list \<Rightarrow> bool"
+  where "constrain_list seen xs = list_all (\<lambda>(g, c_vec). constrain seen g c_vec) xs"
+
+text \<open>group values that follow the rules of an algebraic algorithm are actually in the group\<close>
+lemma constrain_is_in_carrier:
+  assumes "\<forall>g \<in> set seen_vec. g \<in> carrier G"
+  and "constrain seen_vec g c_vec"
+shows "g \<in> carrier G"
+proof -
+  have "g = fold (\<lambda> i acc. acc \<otimes> seen_vec!i [^] (c_vec!i)) [0..<length seen_vec] \<one>"
+    using assms(2) by simp
+  also have "length seen_vec = length c_vec"
+    using assms(2) by fastforce
+  then have "fold (\<lambda> i acc. acc \<otimes> seen_vec!i [^] (c_vec!i)) [0..<length seen_vec] \<one> \<in> carrier G" 
+    using assms(1)
+  proof (induct seen_vec c_vec rule: rev_induct2)
+    case (4 x xs y ys)
+    then have fold_xs_carrier: "fold (\<lambda>i acc. acc \<otimes> xs ! i [^] ys ! i) [0..<length xs] \<one> \<in> carrier G"
+      by fastforce
+    moreover have "x [^] y \<in> carrier G"
+      by (simp add: 4(3))
+    moreover have "fold (\<lambda>i acc. acc \<otimes> (xs @ [x]) ! i [^] (ys @ [y]) ! i) [0..<length (xs @ [x])] \<one> 
+      =  (fold (\<lambda>i acc. acc \<otimes> xs ! i [^] ys ! i) [0..<length xs] \<one>) \<otimes> x [^] y"
+    proof -
+      let ?fyys = "\<lambda>xs::'a list. (\<lambda>i acc. acc \<otimes> xs ! i [^] (ys @ [y]) ! i)"
+      have "fold (\<lambda>i acc. acc \<otimes> (xs @ [x]) ! i [^] (ys @ [y]) ! i) [0..<length (xs @ [x])] \<one> 
+        = fold (?fyys (xs@[x])) [0..<length (xs @ [x])] \<one>" by blast
+      moreover have "\<dots> = (fold (?fyys (xs@[x])) [length (xs @ [x]) - 1] \<circ> fold (?fyys (xs@[x])) [0..<length (xs)]) \<one>"
+        by auto
+      moreover have "\<dots> = ((\<lambda>acc. acc \<otimes> x [^] y)  \<circ> fold (?fyys (xs@[x])) [0..<length (xs)]) \<one>"
+        by (smt (verit, del_insts) "4"(2) One_nat_def add_Suc_right append.right_neutral diff_Suc_Suc diff_zero fold.simps(1) fold_Cons id_comp
+            length_append list.size(3,4) nth_append_length o_apply)
+      moreover have "\<dots> = (fold (?fyys (xs@[x])) [0..<length (xs)] \<one>) \<otimes> x [^] y"
+        by force
+      moreover have "\<dots> = (fold (\<lambda>i acc. acc \<otimes> xs ! i [^] ys ! i) [0..<length (xs)] \<one>) \<otimes> x [^] y"
+      proof - 
+        have "fold (?fyys (xs@[x])) [0..<length (xs)] \<one>
+          = fold (\<lambda>i acc. acc \<otimes> xs ! i [^] ys ! i) [0..<length xs] \<one>"
+        proof(rule fold_cong)
+          fix xa
+          assume "xa \<in> set [0..<length xs]"
+          then have xs_le_xs: "xa < length xs" 
+            by force
+          then have "(xs @ [x]) ! xa = xs ! xa"
+            using nth_append_left by blast
+          moreover have "(ys @ [y]) ! xa = ys ! xa"
+            using 4(2) nth_append_left xs_le_xs by auto
+          ultimately show "(\<lambda>acc. acc \<otimes> (xs @ [x]) ! xa [^] (ys @ [y]) ! xa) = (\<lambda>acc. acc \<otimes> xs ! xa [^] ys ! xa)"
+            by presburger
+        qed force+
+        then show ?thesis by presburger
+      qed
+      ultimately show ?thesis by argo
+    qed
+    ultimately show ?case
+      by auto
+  qed force+
+  finally show "g \<in> carrier G" by blast
+qed
+
 
 ML \<open>
 signature ALGEBRAIC_ALGORITHM =
@@ -13,9 +87,9 @@ val lift_to_algebraicT : typ -> typ -> typ -> typ
 
 val extract_type_params : typ -> string list
 
-val enforce_alg: Name.context -> typ -> term -> term
+val enforce_alg: Name.context -> term -> term -> term
 
-val build_alg_fun : Name.context -> typ -> typ -> term * Name.context
+val build_alg_fun : Name.context -> term -> typ -> term * Name.context
 
 end;
 
@@ -55,7 +129,7 @@ fun create_names_prod_cases nctxt  (Type ("Product_Type.prod", [T1, T2])) =
       val (T2_res,nctxt') = create_names_prod_cases nctxt T2
       val (T1_res, nctxt'') = create_names_prod_cases nctxt' T1
     in 
-      (T1_res@T2_res, nctxt'') (*TODO Is this okay?*)
+      (T1_res@T2_res, nctxt'')
     end
   | create_names_prod_cases nctxt T = 
     let 
@@ -85,24 +159,55 @@ fun extract_vec_pair_list T (Term.Free(t1N,t1T)::Term.Free(t2N,t2T)::xs)
          \<^Const>\<open>list.Nil listT\<close>
       end
 
-fun constrain_pairs nctxt T resT = resT 
-  |> create_names_prod_cases nctxt 
-  |> fst 
-  |> extract_vec_pair_list T
+fun extract_seen_list T (Term.Free(tN,tT)::prams) = 
+  let
+    val pram = Term.Free(tN,tT)
+    val seen = extract_seen_list T prams
+  in
+    if 
+      tT = T
+    then 
+       \<^Const>\<open>List.Cons T for pram seen\<close>
+    else if
+      tT = \<^Type>\<open>list T\<close>
+    then 
+      \<^Const>\<open>append T for pram seen\<close>
+    else 
+      seen
+  end
+  | extract_seen_list T _ = \<^Const>\<open>list.Nil T\<close>
+
+fun get_grpTs grp_desc = 
+  let 
+    fun last_type_arg t = t |> Term.dest_Type_args |> tl |> hd
+    val fst_grpT = Term.fastype_of grp_desc |> Term.dest_Type_args |> hd
+    val snd_grpT = Term.fastype_of grp_desc |> last_type_arg |> last_type_arg |> last_type_arg
+  in 
+    (fst_grpT, snd_grpT)
+  end
+
+fun constrain_pairs nctxt grp_desc resT prams = 
+  let 
+    val (grpT1,grpT2) = get_grpTs grp_desc
+    val xs = resT 
+        |> create_names_prod_cases nctxt 
+        |> fst 
+        |> extract_vec_pair_list grpT1
+    val seen = extract_seen_list grpT1 prams
+  in
+     \<^Const>\<open>cyclic_group.constrain_list grpT1 grpT2 for grp_desc seen xs\<close>
+  end
+
   (* TODO here comes the assert
     add the list of all seen group elements to the parameters here *)
 
-fun create_assert nctxt grpT resT = 
+fun create_assert nctxt grp_desc resT prams = 
   let 
-    val vlist = constrain_pairs nctxt grpT resT
-    val assert_term = @{term True} (* TODO create assert term belongs here *)
+    val _ = writeln (@{make_string} resT);
+    val assert_term = constrain_pairs nctxt grp_desc resT prams
   in 
     \<^Const>\<open>SPMF.assert_spmf for assert_term\<close>
   end
-
-(* TODO create a constrain list pairs function. Accordingly create a type lifting that lifts 'g lists
-to a pair ('g list, int list list) 
-This function should also assert that the lists match in size *)
 
 fun build_ret_term_rec nctxt (Type ("Product_Type.prod", [T1, T2])) = 
   let 
@@ -146,36 +251,32 @@ fun extract_params nctxt T =
     (prams, nctxt') 
   end
 
-fun supply_prams nctxt t = 
-  let  
-    val T = Term.fastype_of t
-    val (prams,nctxt') = extract_params nctxt T
-  in 
-    (rapply prams t, nctxt')
-  end
+fun supply_prams t prams = rapply prams t
 
-fun build_assert_fun nctxt grpT retT t = 
+fun build_assert_fun nctxt grp_desc retT prams t = 
   let 
     val unitT = @{typ unit}
-    val assert_term = create_assert nctxt grpT retT
+    val assert_term = create_assert nctxt grp_desc retT prams
     val t' = Term.absdummy unitT t
   in
    \<^Const>\<open>bind_spmf unitT retT for assert_term t'\<close>
   end
 
-fun build_body_fun nctxt grpT T = 
-  build_ret_term nctxt T |> build_assert_fun nctxt grpT T |> abs_typ_over_term nctxt T
+fun build_body_fun nctxt grp_desc T prams = 
+  build_ret_term nctxt T |> build_assert_fun nctxt grp_desc T prams |> abs_typ_over_term nctxt T
 
-fun enforce_alg nctxt grpT t = 
+fun enforce_alg nctxt grp_desc t = 
   let 
-    val (spmf,nctxt') = supply_prams nctxt t
+    val (prams,nctxt') = Term.fastype_of t |> extract_params nctxt
+    val spmf = supply_prams t prams
     val retT = Term.fastype_of spmf |> strip_spmfT
-    val body_term = build_body_fun nctxt' grpT retT
+    val body_term = build_body_fun nctxt' grp_desc retT prams
+  (* TODO here supply prams as well for seen*)
   in 
      \<^Const>\<open>bind_spmf retT retT for spmf body_term\<close>
   end
 
-fun build_alg_fun nctxt grpT T = 
+fun build_alg_fun nctxt grp_desc T = 
   let
     (* create params to abstract over*)
     val (prams,nctxt') = extract_params nctxt T
@@ -183,130 +284,103 @@ fun build_alg_fun nctxt grpT T =
     val (advN, nctxt'') = Name.variant "\<A>" nctxt'
     val adv = Term.Free(advN,T)
     (* create the fun term to enforce the agm for the adversary *)
-    val fun_term = enforce_alg nctxt grpT adv
+    val fun_term = enforce_alg nctxt grp_desc adv
   in 
     (rabs (rev (adv::prams)) fun_term, nctxt'')
   end
-
-(* TODO write function that takes the free vars list and filters it for group#int_list#xs and 
-  turns it into an Isar level (group*int list) list \<rightarrow> write function that takes the free vars 
-  list, applies the previous described function, and applies create_assert to it.
-
-  Then write a function that takes the free var list and creates prod and abstracts
-
-  Finally put everything together. First create returns spmf, then apply the prod function, then spmf binding. 
-  Once that works, extend with assert.
-*)
 
 end;
 \<close>
 
 ML \<open>
-  Outer_Syntax.local_theory \<^command_keyword>\<open>lift_to_algebraic\<close> "print term test"
-    (Parse.typ -- (Parse.typ -- (Parse.typ -- (\<^keyword>\<open>=>\<close> |--Parse.binding))) >> 
-      (fn (g,(v,(alg,b))) => fn lthy => Local_Theory.raw_theory (fn thy =>
+  Outer_Syntax.local_theory \<^command_keyword>\<open>lift_to_agm\<close> "lift to algebraic type"
+    (Parse.typ -- (Parse.term -- (\<^keyword>\<open>=>\<close> |--Parse.binding)) >> 
+      (fn (alg,(grp,b)) => fn lthy => Local_Theory.raw_theory (fn thy =>
       let
-        val ctxt = Proof_Context.init_global thy;
-        val gT = Syntax.read_typ ctxt g;
-        val vT = Syntax.read_typ ctxt v;
-        val algT = Syntax.read_typ ctxt alg;
-        val agmT = Algebraic_Algorithm.lift_to_algebraicT gT vT algT;
+        val algT = Syntax.read_typ lthy alg;
+        val grp_desc = Syntax.read_term lthy grp;
+        val grpT = Term.fastype_of grp_desc |> Term.dest_Type_args |> hd;
+        val agmT = Algebraic_Algorithm.lift_to_algebraicT grpT @{typ "int list"} algT;
         val tps = Algebraic_Algorithm.extract_type_params agmT;
-        val thy' = Sign.add_type_abbrev ctxt (b, tps, agmT) thy
+        val thy' = Sign.add_type_abbrev lthy (b, tps, agmT) thy
       in thy' end) lthy));
 \<close>
 
+ML \<open>
+  Outer_Syntax.local_theory \<^command_keyword>\<open>AGMtransform\<close> "lift to algebraic type"
+    (Parse.typ -- (Parse.term -- (\<^keyword>\<open>=>\<close> |--Parse.binding)) >> 
+      (fn (adv,(grp,b)) => fn lthy =>
+      let
+        val nctxt = Variable.names_of lthy
+        val advT = Syntax.read_typ lthy adv;
+        val grp_desc = Syntax.read_term lthy grp;
+        val grpT = Term.fastype_of grp_desc |> Term.dest_Type_args |> hd;
+        val agm_advT = Algebraic_Algorithm.lift_to_algebraicT grpT @{typ "int list"} advT;
+        val agm_term = Algebraic_Algorithm.build_alg_fun nctxt grp_desc agm_advT |> fst;
+        val (def, thy') = Local_Theory.define ((b, NoSyn), ((Thm.def_binding b, []), agm_term)) lthy;
+      in thy' end));
+\<close>
 
-context cyclic_group
-begin 
+(*
+ML \<open>
+  Outer_Syntax.local_theory \<^command_keyword>\<open>AGMtransform\<close> "test local definition"
+    (Parse.binding >> (fn b => fn lthy =>
+      let
+        val agmT = @{typ "('g,'b,'a)agm_adv"}
+        val grp_desc = @{term "G"}
+        val agm_term = Algebraic_Algorithm.build_alg_fun Name.context grp_desc agmT |> fst;
+        val (def, lthy') = Local_Theory.define ((b, NoSyn), ((Thm.def_binding b, []), agm_term)) lthy;
+      in lthy' end));
+\<close>*)
 
-fun constrain :: "'a list \<Rightarrow> 'a \<Rightarrow> (int list) \<Rightarrow> bool"
-  where "constrain seen_vec g c_vec = (length seen_vec = length c_vec 
-    \<and> g = fold (\<lambda> i acc. acc \<otimes> seen_vec!i [^] (c_vec!i)) [0..<length seen_vec] \<one>)"
-
-fun constrain_list :: "'a list \<Rightarrow> ('a \<times> nat list) list \<Rightarrow> bool"
-  where "constrain_list seen xs = list_all (\<lambda>(g, c_vec). constrain seen g c_vec) xs"
+subsection \<open>Examples\<close>
 
 type_synonym ('g','b', 'a')alg = "'g' \<Rightarrow> 'b' \<Rightarrow> 'a' \<Rightarrow> ('g' * int*nat) spmf"
 
-lift_to_algebraic 'g "int list"  "('g,'b,'a)cyclic_group.alg" => agm_adv
+lift_to_agm "('a,'b,'g)cyclic_group.alg" G => agm_adv
 
-fun create_assert:: "'x * 'y list \<Rightarrow> bool spmf"
-  where "create_assert (x,y) = return_spmf True"
-
+AGMtransform  "('a,'b,'g)alg" "G" => test_adv
+thm test_adv_def
 
 declare [[ML_print_depth = 1000]]
 ML \<open>
-  val agmT = @{typ "('a,'b,'g)agm_adv"}
+  val agmT = @{typ "('g,'b,'a)agm_adv"}
 
-  val grpT = @{typ 'a}
+  val grp_desc = @{term "G"}
 
-  val test_term = @{term 
-    "\<lambda>(A::('a,'b,'g)agm_adv) g b a. do { 
-      ((g',c),i,j) \<leftarrow> A g b a;
-      _::unit \<leftarrow> assert_spmf(True);
-      return_spmf ((g',c),i,j) 
+  val isabelle_term = @{term 
+    "\<lambda>(A::('g,'b,'a)agm_adv) a b c. do { 
+      ((g,f),e,d) \<leftarrow> A a b c;
+      _::unit \<leftarrow> assert_spmf(constrain_list [a] [(g,f)]);
+      return_spmf ((g,f),e,d) 
     }"}
 
-  val test_monad' = Algebraic_Algorithm.build_alg_fun Name.context grpT agmT |> fst
+  val ml_term = Algebraic_Algorithm.build_alg_fun Name.context grp_desc agmT |> fst
 \<close>
-
-ML \<open>
-  Outer_Syntax.local_theory \<^command_keyword>\<open>local_test\<close> "test local definition"
-    (Parse.binding >> (fn b => fn lthy =>
-      let
-        val agmT = @{typ "('a,'b,'g)agm_adv"}
-        val grpT = @{typ "'a"}
-        val agm_term = Algebraic_Algorithm.build_alg_fun Name.context grpT agmT |> fst;
-        val (def, lthy') = Local_Theory.define ((b, NoSyn), ((Thm.def_binding b, []), agm_term)) lthy;
-      in lthy' end));
-\<close>
-
-declare [[show_types]]
-local_test test_adv
-thm test_adv_def 
 
 definition test 
-  where "test \<equiv> \<lambda>(A::('a,'b,'g)agm_adv) g b a. do { 
-      ((g',c),i,j) \<leftarrow> A g b a;
-      _::unit \<leftarrow>assert_spmf(True);
-      return_spmf ((g',c),i,j) 
-    }" 
+  where "test \<equiv> \<lambda>(A::('g,'b,'a)agm_adv) a b c. do { 
+      ((g,f),e,d) \<leftarrow> A a b c;
+      _::unit \<leftarrow> assert_spmf(constrain_list [a] [(g,f)]);
+      return_spmf ((g,f),e,d) 
+    }"
 
 lemma "test_adv \<equiv> test"
   unfolding test_def test_adv_def
   by argo
 
-end
+type_synonym ('ck', 'commit', 'state') knowledge_soundness_adversary1 = "'ck' \<Rightarrow> ('commit' \<times> 'state') spmf"
 
+type_synonym 'a' vk = "'a' list"
 
-context abstract_polynomial_commitment_scheme
-begin 
+type_synonym 'a' commit = "'a'"
 
-declare [[ML_print_depth = 1000]]
-ML \<open>
- (*
-   val test2 = @{term "\<lambda>(\<A>::('ck, 'commit, 'state, 'argument, 'evaluation, 'witness) 
-  knowledge_soundness_adversary) (E::('r, 'commit, 'trapdoor) extractor). do {
-  let (\<A>1,\<A>2) = \<A>;
-  (ck,vk) \<leftarrow> key_gen;
-  (c,\<sigma>) \<leftarrow> \<A>1 ck;  
-  (p,d) \<leftarrow> E c;             
-  (i, w) \<leftarrow> \<A>2 \<sigma>;                   
-  let (p_i,_) = w;
-  let (p_i',_) = eval ck d p i;         
-  return_spmf (verify_eval vk c i w \<and> p_i \<noteq> p_i')       
-  }"}
-*)
+AGMtransform "('a vk,'a commit,'state)knowledge_soundness_adversary1" "G" => test_adv2
+thm test_adv2_def
+thm test_adv_def
 
-  val test3 =  @{term eval_bind_game}
-  val test4 =  Term.strip_comb (Thm.prop_of @{thm knowledge_soundness_game_def});
-
-  (*val test3 = Term.strip_abs test2;*)
-
-  (*writeln (Syntax.string_of_term  \<^context> test2);*)
-  (*writeln (@{make_string} test2)*)
-\<close>
+(* TODO investigate why lift_to_algebraic 'g  "('a,'b,'g)cyclic_group.alg" => agm_adv 
+changes parameters to ('a * int list)*)
 
 end
 
